\begin{comment}
Part (a)$C_5^3 = \frac{3}{5} = 5 * 4 * 3 (3!) = \frac{5!}{3!(5-2)!}\\ \vspace{1em} = \frac{5!}{3!(5-3)!} = \frac{5*4*3*2*1}{3*2*1, 2*1} = 10$ 3*2*1 cancels
$\frac{k}{n} = \frac{n!}{k!(n-k)!}$

\end{comment}\begin{comment}
Part (a)$C_5^3 = \frac{3}{5} = 5 * 4 * 3 (3!) = \frac{5!}{3!(5-2)!}\\ \vspace{1em} = \frac{5!}{3!(5-3)!} = \frac{5*4*3*2*1}{3*2*1, 2*1} = 10$ 3*2*1 cancels
$\frac{k}{n} = \frac{n!}{k!(n-k)!}$

(This was at the bottom of part a, cant remeber where it goes) 
\\ C_n^k = c_n-1^k-1 + c_{n-1}^{k}$

\end{comment}
